bedrock2/src/bedrock2/WeakestPreconditionProperties.v
@@ -20,6 +20,8 @@ Section WeakestPrecondition.
     match goal with x : X |- _ => induction x end;
     intros.
 
+  (* we prove weakening lemmas for all WP definitions in a syntax-directed fashion,
+   * moving from postcondition towards precondition one logical connective at a time. *)
   Global Instance Proper_literal : Proper (pointwise_relation _ ((pointwise_relation _ Basics.impl) ==> Basics.impl)) WeakestPrecondition.literal.
   Proof. cbv [WeakestPrecondition.literal]; cbv [Proper respectful pointwise_relation Basics.impl]; firstorder idtac. Qed.
 
@@ -204,8 +206,7 @@ Section WeakestPrecondition.
 
   Lemma sound_args : forall m l args mc P,
       WeakestPrecondition.list_map (WeakestPrecondition.expr m l) args P ->
-      exists x mc',
-        Semantics.evaluate_call_args_log m l args mc = Some (x, mc') /\ P x.
+      exists x mc', Semantics.evaluate_call_args_log m l args mc = Some (x, mc') /\ P x.
   Proof.
     induction args; cbn; repeat (subst; t).
     unfold Semantics.eval_expr in *.
